Add typing rules

typing.v
@@ -1,6 +1,6 @@
-From WR Require Import syntax.
-From Coq Require Import ssreflect Sets.Relations_2 Sets.Relations_3 Sets.Relations_3_facts.
-From Hammer Require Import Tactics Hammer.
+From WR Require Import syntax join.
+From Coq Require Import ssreflect.
+From Hammer Require Import Tactics.
 
 Definition context := nat -> tm.
 
@@ -22,157 +22,45 @@ Qed.
 
 Tactic Notation "asimpldep" := repeat (progress (rewrite /dep_ith; asimpl)).
 
-Inductive Par : tm -> tm -> Prop :=
-| P_Var i :
-  (* ------- *)
-  Par (var_tm i) (var_tm i)
-| P_Univ :
+
+Inductive Wt (n : nat) (Γ : context) : tm -> tm -> Prop :=
+| T_Var i :
+  i < n ->
+  (* ------ *)
+  Wt n Γ (var_tm i) (dep_ith Γ i)
+| T_False :
   (* -------- *)
-  Par tUniv tUniv
-| P_False :
-  (* -------- *)
-  Par tFalse tFalse
-| P_Pi A0 A1 B0 B1 :
-  Par A0 A1 ->
-  Par B0 B1 ->
+  Wt n Γ tFalse tUniv
+| T_Pi A B :
+  Wt n Γ A tUniv ->
+  Wt (S n) (A .: Γ) B tUniv ->
   (* --------------------- *)
-  Par (tPi A0 B0) (tPi A1 B1)
-| P_Abs A0 A1 a0 a1 :
-  Par A0 A1 ->
-  Par a0 a1 ->
+  Wt n Γ (tPi A B) tUniv
+| T_Abs A a B :
+  UWf n Γ A ->
+  Wt (S n) (A .: Γ) a B ->
   (* -------------------- *)
-  Par (tAbs A0 a0) (tAbs A1 a1)
-| P_App a0 a1 b0 b1 :
-  Par a0 a1 ->
-  Par b0 b1 ->
-  (* ------------------------- *)
-  Par (tApp a0 b0) (tApp a1 b1)
-| P_AppAbs a A a0 b0 b1 :
-  Par a (tAbs A a0) ->
-  Par b0 b1 ->
-  (* ---------------------------- *)
-  Par (tApp a b0) (subst_tm (b1..) a0).
-
-#[export]Hint Constructors Par : par.
-
-Definition Join := coherent _ Par.
-
-Lemma Par_refl (a : tm) : Par a a.
-Proof. elim : a; hauto lq:on ctrs:Par. Qed.
-
-#[export]Hint Unfold Join : par.
-
-Lemma P_AppAbs' a A a0 b0 b b1 :
-  b = subst_tm (b1..) a0 ->
-  Par a (tAbs A a0) ->
-  Par b0 b1 ->
-  (* ---------------------------- *)
-  Par (tApp a b0) b.
-Proof. hauto lq:on use:P_AppAbs. Qed.
-
-Lemma par_renaming a b (ξ : fin -> fin) :
-  Par a b ->
-  Par (ren_tm ξ a) (ren_tm ξ b).
-  move => h.
-  move : ξ.
-  elim : a b / h => /=; eauto with par.
-  move => *.
-  apply : P_AppAbs'; eauto. by asimpl.
-Qed.
-
-Lemma par_morphing_lift (ξ0 ξ1 : fin -> tm)
-  (h : forall i, Par (ξ0 i) (ξ1 i)) :
-  forall i, Par (up_tm_tm ξ0 i) (up_tm_tm ξ1 i).
-Proof.
-  case => [|i]; first by constructor.
-  asimpl.
-  by apply par_renaming.
-Qed.
-
-Lemma par_morphing a b (ξ0 ξ1 : fin -> tm)
-  (h : forall i, Par (ξ0 i) (ξ1 i)) :
-  Par a b ->
-  Par (subst_tm ξ0 a) (subst_tm ξ1 b).
-Proof.
-  move => h0.
-  move : ξ0 ξ1 h.
-  elim : a b / h0 => /=; eauto with par.
-  - hauto lq:on db:par use:par_morphing_lift.
-  - hauto lq:on db:par use:par_morphing_lift.
-  - move => *; apply : P_AppAbs'; eauto; by asimpl.
-Qed.
-
-Lemma par_cong a0 a1 b0 b1 (h : Par a0 a1) (h1 : Par b0 b1) :
-  Par (subst_tm (b0..) a0) (subst_tm (b1..) a1).
-Proof.
-  apply par_morphing; auto.
-  case; auto.
-  sfirstorder use:Par_refl.
-Qed.
-
-Derive Inversion Par_inv with (forall a b, Par a b).
-
-Lemma par_confluent : Strongly_confluent _ Par.
-Proof.
-  rewrite /Strongly_confluent.
-  move => a b b0 h.
-  move : b0.
-  elim : a b / h.
-  - hauto lq:on inv:Par ctrs:Par.
-  - hauto lq:on inv:Par ctrs:Par.
-  - hauto lq:on inv:Par ctrs:Par.
-  - hauto lq:on inv:Par ctrs:Par.
-  - hauto lq:on inv:Par ctrs:Par.
-  - move => a0 a1 b0 b1 h0 ih0 h1 ih1 b2.
-    elim /Par_inv; try congruence.
-    + qauto l:on ctrs:Par.
-    + move => ? a2 A a3 b3 b4 ? ?.
-      case => *; subst.
-      case /(_ _ ltac:(eassumption)) : ih1 => b [? ?].
-      case /(_ _ ltac:(eassumption)) : ih0 => a [? h2].
-      elim /Par_inv : h2; try congruence.
-      move => ? A0 A1 a2 a4 ? ?.
-      case => *; subst.
-      exists (subst_tm (b..) a4).
-      hauto lq:on ctrs:Par use:par_cong.
-  - move => a A a0 b0 b1 ? ih0 ? ih1 b2.
-    elim /Par_inv; try congruence.
-    + move => h a1 a2 b3 b4 ? ? [*]; subst.
-      case /(_ _ ltac:(eassumption)) : ih0 => a1 [h0 *].
-      case /(_ _ ltac:(eassumption)) : ih1 => b [*].
-      elim /Par_inv : h0; try congruence.
-      move => ? A0 A1 a3 a4 ? ? [*] *; subst.
-      exists (subst_tm (b..) a4).
-      hauto lq:on use:par_cong ctrs:Par.
-    + move => ? a1 A0 a2 b3 b4 ? ? [*] *; subst.
-      case /(_ _ ltac:(eassumption)) : ih0 => a1 [h0 h1].
-      case /(_ _ ltac:(eassumption)) : ih1 => b [*].
-      elim /Par_inv : h0; try congruence.
-      move => ? A1 A2 a3 a4 ? ? [*] *; subst.
-      exists (subst_tm (b..) a4).
-      hauto lq:on use:par_cong ctrs:Par inv:Par.
-Qed.
-
-Lemma pars_confluent : Confluent _ Par.
-Proof.
-  apply Strong_confluence.
-  apply par_confluent.
-Qed.
-
-Lemma Join_reflexive a :
-  Join a a.
-Proof. hauto l:on ctrs:Rstar. Qed.
-
-Lemma Join_symmetric a b :
-  Join a b -> Join b a.
-Proof. sfirstorder use:coherent_symmetric. Qed.
-
-Lemma Join_transitive a b c :
-  Join a b -> Join b c -> Join a c.
-Proof.
-  have := pars_confluent.
-  rewrite /Confluent /confluent /Join /coherent => h [z0 [? h0]] [z1 [h1 ?]].
-  move /(_ b _ _ h0 h1) in h.
-  case : h => z [*].
-  exists z. split; sfirstorder use:Rstar_transitive.
-Qed.
+  Wt n Γ (tAbs A a) (tPi A B)
+| T_App a A B b :
+  Wt n Γ a (tPi A B) ->
+  Wt n Γ b A ->
+  (* -------------------- *)
+  Wt n Γ (tApp a b) (subst_tm (b..) B)
+| T_Conv a A B :
+  Wt n Γ a A ->
+  UWf n Γ B ->
+  Join A B ->
+  (* ----------- *)
+  Wt n Γ a B
+with UWf (n : nat) (Γ : context) : tm -> Prop :=
+| U_Univ :
+  UWf n Γ tUniv
+| U_False :
+  UWf n Γ tFalse
+| U_Pi A B :
+  UWf n Γ A ->
+  UWf (S n) (A .: Γ) B ->
+  UWf n Γ (tPi A B)
+| U_Embed A :
+  Wt n Γ A tUniv ->
+  UWf n Γ A.
