join.v
@@ -1,0 +1,162 @@
+From WR Require Import syntax.
+From Coq Require Import
+  ssreflect
+  Sets.Relations_2
+  Sets.Relations_3
+  Sets.Relations_3_facts.
+From Hammer Require Import Tactics.
+
+Inductive Par : tm -> tm -> Prop :=
+| P_Var i :
+  (* ------- *)
+  Par (var_tm i) (var_tm i)
+| P_Univ :
+  (* -------- *)
+  Par tUniv tUniv
+| P_False :
+  (* -------- *)
+  Par tFalse tFalse
+| P_Pi A0 A1 B0 B1 :
+  Par A0 A1 ->
+  Par B0 B1 ->
+  (* --------------------- *)
+  Par (tPi A0 B0) (tPi A1 B1)
+| P_Abs A0 A1 a0 a1 :
+  Par A0 A1 ->
+  Par a0 a1 ->
+  (* -------------------- *)
+  Par (tAbs A0 a0) (tAbs A1 a1)
+| P_App a0 a1 b0 b1 :
+  Par a0 a1 ->
+  Par b0 b1 ->
+  (* ------------------------- *)
+  Par (tApp a0 b0) (tApp a1 b1)
+| P_AppAbs a A a0 b0 b1 :
+  Par a (tAbs A a0) ->
+  Par b0 b1 ->
+  (* ---------------------------- *)
+  Par (tApp a b0) (subst_tm (b1..) a0).
+
+#[export]Hint Constructors Par : par.
+
+Definition Join := coherent _ Par.
+
+Lemma Par_refl (a : tm) : Par a a.
+Proof. elim : a; hauto lq:on ctrs:Par. Qed.
+
+#[export]Hint Unfold Join : par.
+
+Lemma P_AppAbs' a A a0 b0 b b1 :
+  b = subst_tm (b1..) a0 ->
+  Par a (tAbs A a0) ->
+  Par b0 b1 ->
+  (* ---------------------------- *)
+  Par (tApp a b0) b.
+Proof. hauto lq:on use:P_AppAbs. Qed.
+
+Lemma par_renaming a b (ξ : fin -> fin) :
+  Par a b ->
+  Par (ren_tm ξ a) (ren_tm ξ b).
+  move => h.
+  move : ξ.
+  elim : a b / h => /=; eauto with par.
+  move => *.
+  apply : P_AppAbs'; eauto. by asimpl.
+Qed.
+
+Lemma par_morphing_lift (ξ0 ξ1 : fin -> tm)
+  (h : forall i, Par (ξ0 i) (ξ1 i)) :
+  forall i, Par (up_tm_tm ξ0 i) (up_tm_tm ξ1 i).
+Proof.
+  case => [|i]; first by constructor.
+  asimpl.
+  by apply par_renaming.
+Qed.
+
+Lemma par_morphing a b (ξ0 ξ1 : fin -> tm)
+  (h : forall i, Par (ξ0 i) (ξ1 i)) :
+  Par a b ->
+  Par (subst_tm ξ0 a) (subst_tm ξ1 b).
+Proof.
+  move => h0.
+  move : ξ0 ξ1 h.
+  elim : a b / h0 => /=; eauto with par.
+  - hauto lq:on db:par use:par_morphing_lift.
+  - hauto lq:on db:par use:par_morphing_lift.
+  - move => *; apply : P_AppAbs'; eauto; by asimpl.
+Qed.
+
+Lemma par_cong a0 a1 b0 b1 (h : Par a0 a1) (h1 : Par b0 b1) :
+  Par (subst_tm (b0..) a0) (subst_tm (b1..) a1).
+Proof.
+  apply par_morphing; auto.
+  case; auto.
+  sfirstorder use:Par_refl.
+Qed.
+
+Derive Inversion Par_inv with (forall a b, Par a b).
+
+Lemma par_confluent : Strongly_confluent _ Par.
+Proof.
+  rewrite /Strongly_confluent.
+  move => a b b0 h.
+  move : b0.
+  elim : a b / h.
+  - hauto lq:on inv:Par ctrs:Par.
+  - hauto lq:on inv:Par ctrs:Par.
+  - hauto lq:on inv:Par ctrs:Par.
+  - hauto lq:on inv:Par ctrs:Par.
+  - hauto lq:on inv:Par ctrs:Par.
+  - move => a0 a1 b0 b1 h0 ih0 h1 ih1 b2.
+    elim /Par_inv; try congruence.
+    + qauto l:on ctrs:Par.
+    + move => ? a2 A a3 b3 b4 ? ?.
+      case => *; subst.
+      case /(_ _ ltac:(eassumption)) : ih1 => b [? ?].
+      case /(_ _ ltac:(eassumption)) : ih0 => a [? h2].
+      elim /Par_inv : h2; try congruence.
+      move => ? A0 A1 a2 a4 ? ?.
+      case => *; subst.
+      exists (subst_tm (b..) a4).
+      hauto lq:on ctrs:Par use:par_cong.
+  - move => a A a0 b0 b1 ? ih0 ? ih1 b2.
+    elim /Par_inv; try congruence.
+    + move => h a1 a2 b3 b4 ? ? [*]; subst.
+      case /(_ _ ltac:(eassumption)) : ih0 => a1 [h0 *].
+      case /(_ _ ltac:(eassumption)) : ih1 => b [*].
+      elim /Par_inv : h0; try congruence.
+      move => ? A0 A1 a3 a4 ? ? [*] *; subst.
+      exists (subst_tm (b..) a4).
+      hauto lq:on use:par_cong ctrs:Par.
+    + move => ? a1 A0 a2 b3 b4 ? ? [*] *; subst.
+      case /(_ _ ltac:(eassumption)) : ih0 => a1 [h0 h1].
+      case /(_ _ ltac:(eassumption)) : ih1 => b [*].
+      elim /Par_inv : h0; try congruence.
+      move => ? A1 A2 a3 a4 ? ? [*] *; subst.
+      exists (subst_tm (b..) a4).
+      hauto lq:on use:par_cong ctrs:Par inv:Par.
+Qed.
+
+Lemma pars_confluent : Confluent _ Par.
+Proof.
+  apply Strong_confluence.
+  apply par_confluent.
+Qed.
+
+Lemma Join_reflexive a :
+  Join a a.
+Proof. hauto l:on ctrs:Rstar. Qed.
+
+Lemma Join_symmetric a b :
+  Join a b -> Join b a.
+Proof. sfirstorder use:coherent_symmetric. Qed.
+
+Lemma Join_transitive a b c :
+  Join a b -> Join b c -> Join a c.
+Proof.
+  have := pars_confluent.
+  rewrite /Confluent /confluent /Join /coherent => h [z0 [? h0]] [z1 [h1 ?]].
+  move /(_ b _ _ h0 h1) in h.
+  case : h => z [*].
+  exists z. split; sfirstorder use:Rstar_transitive.
+Qed.
